autoclrs/ch07-quicksort/CLRS.Ch07.Partition.Impl.fsti
@@ -49,6 +49,7 @@ fn clrs_partition_wrapper_with_ticks
       lb <= Seq.index s_pivot 0 /\ Seq.index s_pivot 0 <= rb /\
       between_bounds s1 lb (Seq.index s_pivot 0) /\
       between_bounds s2 (Seq.index s_pivot 0) rb /\
+      strictly_larger_than s2 (Seq.index s_pivot 0) /\
       permutation s0 (Seq.append s1 (Seq.append s_pivot s2)) /\
       complexity_exact_linear cf (reveal c0) (hi - lo - 1)
    ))
